theories/properties.v
@@ -2,8 +2,7 @@
 
 From Wasm Require Export datatypes_properties operations typing opsem common.
 From mathcomp Require Import ssreflect ssrfun ssrnat ssrbool eqtype seq.
-From StrongInduction Require Import StrongInduction.
-From Coq Require Import Bool Program.Equality.
+From Coq Require Import Bool Program.Equality Wf_nat.
 
 Set Implicit Arguments.
 Unset Strict Implicit.
@@ -759,47 +758,45 @@ Proof.
     by apply IHl1.
 Qed.
 
+Fixpoint ai_gen_measure (e: administrative_instruction) : nat :=
+   match e with
+   | AI_label _ _ es => 1 + List.list_max (map ai_gen_measure es)
+   | _ => 0
+   end.
 
 (** The decreasing measure used in the definition of [lfilled_pickable_rec_gen]. **)
-Definition lfilled_pickable_rec_gen_measure (LI : seq administrative_instruction) :=
-  TProp.max
-    (seq_administrative_instruction_rect'
-       (fun _ => 0)
-       0
-       (fun _ => 0)
-       (fun _ LI1 LI2 m1 m2 => 1 + TProp.max m2)
-       (fun _ _ LI' m => 0)
-       (fun _ _ _ => 0)
-       LI).
-
+ Definition lfilled_pickable_rec_gen_measure (LI: list administrative_instruction) : nat :=
+   List.list_max (map ai_gen_measure LI).
+ 
 Lemma lfilled_pickable_rec_gen_measure_cons : forall I LI,
   lfilled_pickable_rec_gen_measure LI <= lfilled_pickable_rec_gen_measure (I :: LI).
 Proof.
-  move=> I LI. by apply: leq_maxr.
+  move=> I LI.
+  unfold lfilled_pickable_rec_gen_measure => /=.
+  by lias.
 Qed.
 
 Lemma lfilled_pickable_rec_gen_measure_concat_l : forall LI1 LI2,
   lfilled_pickable_rec_gen_measure LI1 <= lfilled_pickable_rec_gen_measure (LI1 ++ LI2).
 Proof.
-  move => LI1 LI2. induction LI1 => /=.
-  - rewrite {1} /lfilled_pickable_rec_gen_measure /=. by lias.
-  - rewrite /lfilled_pickable_rec_gen_measure /=.
-    by apply: maxn_congruence_r.
+  unfold lfilled_pickable_rec_gen_measure => /=.
+  move => LI1 LI2. rewrite map_cat List.list_max_app.
+  by lias.
 Qed.
 
 Lemma lfilled_pickable_rec_gen_measure_concat_r : forall LI1 LI2,
   lfilled_pickable_rec_gen_measure LI2 <= lfilled_pickable_rec_gen_measure (LI1 ++ LI2).
 Proof.
-  move => LI1 LI2. induction LI1 => /=.
-  - rewrite {1} /lfilled_pickable_rec_gen_measure /=. by lias.
-  - rewrite /lfilled_pickable_rec_gen_measure /=. eapply leq_trans; first by apply: IHLI1.
-    by apply: leq_maxr.
+  unfold lfilled_pickable_rec_gen_measure => /=.
+  move => LI1 LI2. rewrite map_cat List.list_max_app.
+  by lias.
 Qed.
 
 Lemma lfilled_pickable_rec_gen_measure_label_r : forall n es LI LI',
   lfilled_pickable_rec_gen_measure LI < lfilled_pickable_rec_gen_measure (AI_label n es LI :: LI').
 Proof.
-  move=> n es LI LI'. rewrite /lfilled_pickable_rec_gen_measure /=. by apply: leq_maxl.
+  move=> n es LI LI'. rewrite /lfilled_pickable_rec_gen_measure /=.
+  destruct (List.list_max (map ai_gen_measure LI')); by lias.
 Qed.
 
 (** A helper definition for [lfilled_decidable_rec]. **)
@@ -811,7 +808,7 @@ Proof.
   apply: (@pickable2_equiv _ _ (fun n lh => lfilledInd n lh (fes (0+n) lh) es')); first by [].
   move: 0 => k.
   have [m E]: { m | lfilled_pickable_rec_gen_measure es' = m }; first by eexists.
-  move: fes D0 es' E k. strong induction m. rename X into IH. move=> fes D0 es' E k.
+  move: fes D0 es' E k. induction (lt_wf m) as [m _ H]. rename H into IH. move=> fes D0 es' E k.
   have Dcl: forall vs, decidable (const_list vs).
   { move=> vs. by apply: is_true_decidable. }
   (** First, we check whether we can set [n = 0]. **)
