theories/datatypes_properties.v
@@ -303,11 +303,13 @@ Definition administrative_instruction_ind' (P : administrative_instruction -> Pr
 
 (** Administrative instructions frequently come in lists.
   Here is the corresponding induction principle. **)
+(*
 Definition seq_administrative_instruction_rect' :=
   ltac:(rect'_build_list administrative_instruction_rect).
 
 Definition seq_administrative_instruction_ind' (P : administrative_instruction -> Prop) :=
   @seq_administrative_instruction_rect' P.
+*)
 
 Definition administrative_instruction_eq_dec : forall e1 e2 : administrative_instruction,
   {e1 = e2} + {e1 <> e2}.
