README.md
@@ -1,86 +1,19 @@
+# coq_iris_wasm
+This branch contains the work on the Iris-Wasm Program Logic, which is the artifact for the paper
+*Iris-Wasm: Robust and Modular Verification of WebAssembly Programs* on PLDI'23.
+
+This version is slightly adapted from the submitted artefact, providing an `opam` build instead of the submitted `esy` build. 
+The old `esy` build can still be found on the branch `iris-wasm-native`, or on Zenodo at https://zenodo.org/records/7808708.
+
+# Installation and Compilation
+
+The project can be installed using opam.
+
+Compiling the dependencies requires having at least 4-8 GB of RAM on your computer.
+```bash
+opam repo add coq-released https://coq.inria.fr/opam/released
+opam install .
+```
+
 # Usage
-
-## Installation and Compilation
-
-The project comes with an `esy` packaging.
-
-The following programs are assumed to be installed: `git`, `curl`, `m4`, `autoconf`, and `automake`.
-These programs are used to fetch and compile dependencies.
-
-Installing `esy` itself can be done through `npm`.
-It should then look like something like that:
-```bash
-sudo apt install npm git curl m4 autoconf
-sudo npm install --global esy@latest # Tested with version 0.6.12 of esy.
-```
-Note that despite using `npm` to be installed, `esy` is not JavaScript-based.
-If you prefer to avoid `npm` altogether, there are other ways to install `esy`: see <https://esy.sh/> for more information.
-
-Once `esy` is installed, simply type `esy` to download and install the dependencies and compile everything.
-```bash
-esy
-```
-
-Compiling the dependencies may require at least 16GB of RAM.
-
-## Troubleshooting
-
-- On MacOS Monterey, it is required to use at least esy >=0.6.12 as there is a sandboxing bug for versions below that.
-
-- Due to compatibility issues of several dependencies, the codebase currently fails to build on any OS using glibc >= 2.34.
-
-## Editing the Project
-
-Type `esy shell` to open a shell with the right compilation environment.
-You can also type `esy emacs theories/wasm.v` to open Emacs with the right environment (assuming that Emacs is installed with Proof General in your system).
-Note that `emacs theories/wasm.v` (without the `esy` prefix) will open Emacs without setting the local dependencies: doing so will likely prevent `coq` from finding the needed dependencies.
-
-To use CoqIDE in this developpment, you first need to install its system dependencies (these are probably already installed on your system if you are using CoqIDE):
-```bash
-sudo apt install libcairo2-dev libexpat1-dev libgtk-3-dev libgtksourceview-3.0-dev
-```
-Then, replace the line `devDependencies: {},` by `devDependencies: {"@opam/coqide": "*"}` in [package.json](./package.json), and run `esy` again.
-Typing `esy coqide theories/wasm.v` should now work.
-
-To use VSCode in this development, a [.vscode/settings.json](.vscode/settings.json) needs to be generated first: this file enables VSCode to know where the dependencies are stored in your system.
-It can be generated with `esy vscode`.
-
-The [tests](./tests) folder contains Markdown files checked by `mdx` during the continuous intergration.
-
-## Using the project
-
-A file `wasm_interpreter` will have been generated.
-It takes as argument a list of Wasm files, followed by a function name, followed by a depth.
-For instance, to interpret the function `hello` defined in [tests/const.wasm](tests/const.wasm), run:
-```bash
-./wasm_interpreter tests/const.wasm hello 10
-```
-The interpreter can display intermediate states of the operational semantics:
-```bash
-./wasm_interpreter tests/const.wasm hello 10 --vi
-```
-for example
-```
-step 1:
-normal
-  local 1
-  with values (empty)
-    block i32
-        i32.const 42
-    end
-  end local
-with values (empty)
-and store unchanged
-
-step 2:
-normal
-  local 1
-  with values (empty)
-    label 1
-    label_cont
-      i32.const 42
-    end label
-  end local
-with values (empty)
-and store unchanged
-```
+For detailed usage, check the Readme file attached on the artifact submission at https://zenodo.org/records/7808708.
